compiler/backend/proofs/stack_rawcallProofScript.sml
@@ -1,0 +1,676 @@
+(*
+  Correctness proof for stack_rawcall
+*)
+
+open preamble stackLangTheory stackSemTheory stackPropsTheory stack_rawcallTheory
+local open wordSemTheory labPropsTheory in end
+
+val _ = new_theory"stack_rawcallProof";
+val _ = (max_print_depth := 18);
+
+val word_shift_def = backend_commonTheory.word_shift_def
+val theWord_def = wordSemTheory.theWord_def;
+val isWord_def = wordSemTheory.isWord_def;
+
+val _ = set_grammar_ancestry["stack_rawcall","stackLang","stackSem","stackProps"];
+Overload good_dimindex[local] = ``labProps$good_dimindex``
+Overload comp[local] = ``stack_rawcall$comp``
+Overload compile[local] = ``stack_rawcall$compile``
+
+Definition state_ok_def:
+  state_ok i code <=>
+    !n v.
+      lookup n i = SOME v ==>
+      ?p. lookup n code = SOME (Seq (StackAlloc v) p)
+End
+
+Definition state_rel_def:
+  state_rel cc co i s t <=>
+    ?c.
+      domain c = domain s.code /\
+      t = s with <| code := c ;
+                    compile := cc ;
+                    compile_oracle := co
+                  |> /\
+      state_ok i s.code /\
+      !n b.
+        lookup n s.code = SOME b ==>
+        ?i. state_ok i s.code /\
+            lookup n c = SOME (comp_top i b)
+End
+
+Theorem state_rel_thm =
+  state_rel_def |> SIMP_RULE (srw_ss()) [state_component_equality];
+
+Theorem comp_correct:
+   !p (s:('a,'c,'b)stackSem$state) t i r s1.
+     evaluate (p,s) = (r,s1) /\ r <> SOME Error /\ state_rel cc co i s t
+     ==>
+     (?ck t1 k1.
+        state_rel cc co i s1 t1 /\
+        evaluate (stack_rawcall$comp_top i p,t with clock := t.clock + ck) =
+          (r,t1 with stack_space := k1) /\
+        (r <> SOME TimeOut /\ r <> SOME (Halt (Word 2w)) ==> k1 = t1.stack_space)) /\
+     (?ck t1 k1.
+        state_rel cc co i s1 t1 /\
+        evaluate (stack_rawcall$comp i p,t with clock := t.clock + ck) =
+          (r,t1 with stack_space := k1) /\
+        (r <> SOME TimeOut /\ r <> SOME (Halt (Word 2w)) ==> k1 = t1.stack_space))
+Proof
+  recInduct evaluate_ind \\ rpt conj_tac \\ rpt gen_tac
+  \\ strip_tac \\ simp [comp_top_def]
+  THEN1
+   (rename [`Skip`]
+    \\ simp [comp_top_def,comp_def]
+    \\ fs [evaluate_def] \\ rveq \\ fs []
+    \\ qexists_tac `0`
+    \\ qexists_tac `t` \\ fs [state_component_equality])
+  THEN1
+   (rename [`Halt`]
+    \\ simp [comp_top_def,comp_def]
+    \\ fs [evaluate_def] \\ rveq \\ fs []
+    \\ fs [state_rel_def] \\ rveq \\ fs [get_var_def,CaseEq"option"]
+    \\ rveq \\ fs [PULL_EXISTS] \\ cheat)
+  THEN1
+   (rename [`Alloc`] \\ cheat)
+  THEN1
+   (rename [`Inst`] \\ cheat)
+  THEN1
+   (rename [`Get`] \\ cheat)
+  THEN1
+   (rename [`Set`] \\ cheat)
+  THEN1
+   (rename [`Tick`] \\ cheat)
+  THEN1
+   (rename [`Seq`]
+    \\ rpt gen_tac \\ strip_tac
+    \\ conj_asm1_tac THEN1
+     (fs [evaluate_def] \\ rpt (pairarg_tac \\ fs [])
+      \\ reverse (fs [CaseEq"bool"]) \\ rveq \\ fs []
+      THEN1
+       (first_x_assum drule \\ strip_tac \\ fs []
+        \\ qexists_tac `ck'` \\ fs [] \\ metis_tac [])
+      \\ first_x_assum drule \\ rewrite_tac [GSYM AND_IMP_INTRO]
+      \\ disch_then kall_tac \\ strip_tac
+      \\ first_x_assum drule \\ rewrite_tac [GSYM AND_IMP_INTRO]
+      \\ disch_then kall_tac \\ strip_tac
+      \\ `t1 with stack_space := t1.stack_space = t1` by fs [state_component_equality]
+      \\ fs []
+      \\ qpat_x_assum `evaluate (comp i c1,_) = (NONE,_)` assume_tac
+      \\ drule evaluate_add_clock \\ fs []
+      \\ disch_then (qspec_then `ck'` assume_tac)
+      \\ qexists_tac `ck + ck'` \\ fs []
+      \\ asm_exists_tac \\ simp [state_component_equality])
+    \\ Cases_on `comp i (Seq c1 c2) = Seq (comp i c1) (comp i c2)`
+    THEN1 asm_rewrite_tac []
+    \\ fs [] \\ simp [comp_top_def]
+    \\ ntac 1 (pop_assum mp_tac)
+    \\ simp [Q.SPECL[`Seq c1 c2`] comp_def]
+    \\ simp [comp_seq_def]
+    \\ simp [CaseEq"option",pair_case_eq,FORALL_PROD,PULL_EXISTS]
+    \\ Cases_on `dest_case (c1,c2)` \\ fs []
+    \\ PairCases_on `x` \\ fs []
+    \\ Cases_on `lookup x1 i` \\ fs []
+    \\ disch_then kall_tac
+    \\ fs [dest_case_def,CaseEq"stackLang$prog",CaseEq"option",CaseEq"sum"]
+    \\ rveq \\ fs []
+    \\ qpat_x_assum `evaluate _ = _` kall_tac
+    \\ qpat_x_assum `evaluate _ = _` mp_tac
+    \\ qpat_x_assum `!x. _` kall_tac
+    \\ simp [evaluate_def]
+    \\ IF_CASES_TAC \\ fs []
+    \\ IF_CASES_TAC \\ fs [find_code_def]
+    \\ qpat_assum `state_rel cc co i s t` (mp_tac o REWRITE_RULE [state_rel_thm])
+    \\ strip_tac
+    \\ qpat_assum `state_ok i _` (mp_tac o REWRITE_RULE [state_ok_def])
+    \\ disch_then drule \\ strip_tac
+    \\ first_assum drule
+    \\ strip_tac \\ fs []
+    \\ IF_CASES_TAC \\ fs [] \\ rveq
+    \\ Cases_on `s.clock = 0` \\ fs []
+    THEN1
+     (rpt strip_tac \\ rveq \\ fs []
+      \\ qexists_tac `0` \\ fs []
+      \\ simp [state_rel_def,PULL_EXISTS]
+      \\ asm_exists_tac \\ simp [empty_env_def]
+      \\ rw [] \\ fs [] \\ simp [evaluate_def,dest_Seq_def,comp_top_def,empty_env_def]
+      \\ fs [state_component_equality,empty_env_def])
+    \\ fs [dec_clock_def]
+    \\ last_x_assum mp_tac
+    \\ simp [Once evaluate_def]
+    \\ simp [Once evaluate_def,find_code_def,dec_clock_def]
+    \\ TOP_CASE_TAC \\ Cases_on `q` \\ fs []
+    \\ rpt strip_tac \\ rveq \\ fs [] \\ rfs []
+    \\ `state_rel t.compile t.compile_oracle i
+           (s with stack_space := k + s.stack_space)
+           (t with stack_space := k + t.stack_space)`
+         by fs [state_rel_thm]
+    \\ first_x_assum drule
+    \\ rewrite_tac [GSYM AND_IMP_INTRO]
+    \\ disch_then kall_tac
+    \\ simp[Once comp_def]
+    \\ simp [Once evaluate_def,find_code_def,dec_clock_def,comp_top_def]
+    \\ simp[Once comp_def]
+    \\ strip_tac
+    \\ asm_exists_tac \\ simp []
+    \\ rw []
+    THEN1
+     (simp [Once evaluate_def,comp_top_def,dest_Seq_def,dec_clock_def]
+      \\ qexists_tac `ck` \\ fs []
+      \\ once_rewrite_tac [CONJ_COMM] \\ asm_exists_tac \\ simp []
+      \\ ntac 2 (pop_assum mp_tac)
+      \\ simp [evaluate_def]
+      \\ qpat_abbrev_tac `pat1 = (comp i' p, _)`
+      \\ qpat_abbrev_tac `pat2 = (comp i' p, _)`
+      \\ qsuff_tac `pat1 = pat2` \\ fs []
+      \\ unabbrev_all_tac \\ fs [state_component_equality])
+    THEN1
+     (simp [evaluate_def]
+      \\ simp [comp_top_def,dest_Seq_def,dec_clock_def]
+      \\ qexists_tac `ck` \\ fs []
+      \\ once_rewrite_tac [CONJ_COMM] \\ asm_exists_tac \\ simp []
+      \\ qpat_x_assum `_ = (_,_)` mp_tac
+      \\ simp [evaluate_def])
+    THEN1
+     (simp [evaluate_def]
+      \\ simp [comp_top_def,dest_Seq_def,dec_clock_def]
+      \\ qpat_x_assum `_ = (_,_)` mp_tac
+      (* \\ qpat_x_assum `_ = (_,_)` mp_tac *)
+      \\ simp [evaluate_def]
+      \\ `k + s.stack_space < x <=> s.stack_space < x - k` by fs []
+      \\ asm_rewrite_tac [] \\ pop_assum kall_tac
+      \\ IF_CASES_TAC \\ fs [empty_env_def]
+      THEN1
+       (rw [] \\ fs [state_component_equality,empty_env_def]
+        \\ qexists_tac `ck` \\ fs [])
+      \\ simp [dest_Seq_def,comp_top_def]
+      \\ TOP_CASE_TAC \\ fs []
+      \\ TOP_CASE_TAC \\ fs []
+      \\ strip_tac \\ rveq \\ fs []
+      \\ qexists_tac `ck + 1` \\ fs []
+      \\ once_rewrite_tac [CONJ_COMM] \\ asm_exists_tac \\ simp []))
+  THEN1
+   (rename [`Return`] \\ cheat)
+  THEN1
+   (rename [`Raise`] \\ cheat)
+  THEN1
+   (rename [`If`] \\ cheat)
+  THEN1
+   (rename [`While`] \\ cheat)
+  THEN1
+   (rename [`JumpLower`] \\ cheat)
+  THEN1
+   (rename [`RawCall`] \\ cheat)
+  THEN1
+   (rename [`Call`] \\ cheat)
+  THEN1
+   (rename [`Install`] \\ cheat)
+  THEN1
+   (rename [`CodeBufferWrite`] \\ cheat)
+  THEN1
+   (rename [`DataBufferWrite`] \\ cheat)
+  THEN1
+   (rename [`FFI`] \\ cheat)
+  THEN1
+   (rename [`LocValue`] \\ cheat)
+  THEN1
+   (rename [`StackAlloc`] \\ cheat)
+  THEN1
+   (rename [`StackFree`] \\ cheat)
+  THEN1
+   (rename [`StackLoad`] \\ cheat)
+  THEN1
+   (rename [`StackLoadAny`] \\ cheat)
+  THEN1
+   (rename [`StackStore`] \\ cheat)
+  THEN1
+   (rename [`StackStoreAny`] \\ cheat)
+  THEN1
+   (rename [`StackGetSize`] \\ cheat)
+  THEN1
+   (rename [`StackSetSize`] \\ cheat)
+  THEN1
+   (rename [`BitmapLoad`] \\ cheat)
+QED
+
+(*
+
+Theorem compile_semantics:
+   s.use_stack ∧
+   semantics start s <> Fail
+   ==>
+   semantics start (s with <|
+                      code := fromAList (stack_rawcall$compile (toAList s.code));
+                      compile := cc;
+                      compile_oracle := (I ## compile ## I) o s.compile_oracle |>) =
+   semantics start s
+Proof
+  simp[GSYM AND_IMP_INTRO] >> ntac 6 strip_tac >>
+  simp[semantics_def] >>
+  IF_CASES_TAC >> full_simp_tac(srw_ss())[] >>
+  DEEP_INTRO_TAC some_intro >> full_simp_tac(srw_ss())[] >>
+  conj_tac >- (
+    gen_tac >> ntac 2 strip_tac >>
+    IF_CASES_TAC >> full_simp_tac(srw_ss())[] >- (
+      first_x_assum(qspec_then`k'`mp_tac)>>simp[]>>
+      (fn g => subterm (fn tm => Cases_on`^(assert has_pair_type tm)`) (#2 g) g) >>
+      simp[] >>
+      qmatch_assum_rename_tac`_ = (res,_)` >>
+      Cases_on`res=SOME Error`>>simp[]>>
+      drule comp_correct_thm >>
+      simp[alloc_arg_def,RIGHT_FORALL_IMP_THM] >>
+      impl_tac >- metis_tac[] >>
+      simp[comp_def] >>
+      strip_tac >>
+      qpat_x_assum`_ ≠ SOME TimeOut`mp_tac >>
+      (fn g => subterm (fn tm => Cases_on`^(assert has_pair_type tm)`) (#2 g) g) >>
+      strip_tac >>
+      drule (Q.GEN`extra`evaluate_add_clock) >>
+      disch_then(qspec_then`ck`mp_tac) >> full_simp_tac(srw_ss())[] >>
+      fs[]) >>
+    DEEP_INTRO_TAC some_intro >> full_simp_tac(srw_ss())[] >>
+    conj_tac >- (
+      srw_tac[][] >>
+      Cases_on`r=TimeOut`>>full_simp_tac(srw_ss())[]>>
+      qpat_x_assum `evaluate _ = (SOME r, t)` assume_tac >>
+      old_dxrule comp_correct_thm >>
+      simp[RIGHT_FORALL_IMP_THM] >>
+      impl_tac >- (
+        simp[alloc_arg_def] >>
+        reverse conj_tac >- metis_tac[] >>
+        CCONTR_TAC >> fs[]) >>
+      strip_tac >>
+      old_dxrule(GEN_ALL evaluate_add_clock) >>
+      disch_then(qspec_then `k'` mp_tac) >>
+      impl_tac >- (CCONTR_TAC >> fs[]) >>
+      dxrule evaluate_add_clock >>
+      disch_then(qspec_then `ck + k` mp_tac) >>
+      impl_tac >- (CCONTR_TAC >> fs[]) >>
+      ntac 2 strip_tac >>
+      fs[comp_def,state_component_equality] >>
+      rveq >> rpt(PURE_FULL_CASE_TAC >> fs[])) >>
+    drule comp_correct_thm >>
+    simp[RIGHT_FORALL_IMP_THM] >>
+    impl_tac >- (
+      simp[alloc_arg_def] >>
+      reverse conj_tac >- metis_tac[] >>
+      rpt(first_x_assum(qspec_then`k`mp_tac)) >>
+    srw_tac[][]) >>
+    simp[comp_def] >>
+    strip_tac >>
+    asm_exists_tac >> simp[] >>
+    BasicProvers.TOP_CASE_TAC >> full_simp_tac(srw_ss())[] >>
+    BasicProvers.TOP_CASE_TAC >> full_simp_tac(srw_ss())[]) >>
+  ntac 2 strip_tac >>
+  IF_CASES_TAC >> full_simp_tac(srw_ss())[] >- (
+    first_x_assum(qspec_then`k`mp_tac)>>simp[]>>
+    first_x_assum(qspec_then`k`mp_tac)>>
+    (fn g => subterm (fn tm => Cases_on`^(assert has_pair_type tm)`) (#2 g) g) >>
+    simp[] >> strip_tac >> fs[] >>
+    drule comp_correct_thm >>
+    simp[alloc_arg_def,comp_def] >>
+    conj_tac >- metis_tac[] >>
+    srw_tac[][] >>
+    qpat_x_assum`_ ≠ SOME TimeOut`mp_tac >>
+    (fn g => subterm (fn tm => Cases_on`^(assert has_pair_type tm)`) (#2 g) g) >> srw_tac[][] >>
+    drule (GEN_ALL evaluate_add_clock) >>
+    disch_then(qspec_then`ck`mp_tac)>>simp[]) >>
+  DEEP_INTRO_TAC some_intro >> full_simp_tac(srw_ss())[] >>
+  conj_tac >- (
+    srw_tac[][] >>
+    qpat_x_assum`∀k t. _`(qspec_then`k`mp_tac) >>
+    (fn g => subterm (fn tm => Cases_on`^(assert has_pair_type tm)`) (#2 g) g) >>
+    simp[] >>
+    last_x_assum mp_tac >>
+    last_x_assum mp_tac >>
+    last_x_assum(qspec_then`k`mp_tac) >>
+    srw_tac[][] >> full_simp_tac(srw_ss())[] >>
+    drule comp_correct_thm >>
+    simp[alloc_arg_def,comp_def] >>
+    conj_tac >- metis_tac[] >>
+    srw_tac[][] >>
+    Cases_on`r=TimeOut`>>full_simp_tac(srw_ss())[] >>
+    qhdtm_x_assum`evaluate`mp_tac >>
+    drule (GEN_ALL evaluate_add_clock) >>
+    disch_then(qspec_then`ck`mp_tac)>>simp[] ) >>
+  srw_tac[][] >>
+  qmatch_abbrev_tac`build_lprefix_lub l1 = build_lprefix_lub l2` >>
+  `(lprefix_chain l1 ∧ lprefix_chain l2) ∧ equiv_lprefix_chain l1 l2`
+    suffices_by metis_tac[build_lprefix_lub_thm,lprefix_lub_new_chain,unique_lprefix_lub] >>
+  conj_asm1_tac >- (
+    UNABBREV_ALL_TAC >>
+    conj_tac >>
+    Ho_Rewrite.ONCE_REWRITE_TAC[GSYM o_DEF] >>
+    REWRITE_TAC[IMAGE_COMPOSE] >>
+    match_mp_tac prefix_chain_lprefix_chain >>
+    simp[prefix_chain_def,PULL_EXISTS] >>
+    qx_genl_tac[`k1`,`k2`] >>
+    qspecl_then[`k1`,`k2`]mp_tac LESS_EQ_CASES >>
+    match_mp_tac(PROVE[]``((a ⇒ c) ∧ (b ⇒ d)) ⇒ (a ∨ b ⇒ c ∨ d)``) \\
+    simp[LESS_EQ_EXISTS] \\
+    conj_tac \\ strip_tac \\ rveq \\
+    qmatch_goalsub_abbrev_tac`e,ss` \\
+    Q.ISPECL_THEN[`p`,`e`,`ss`]mp_tac(GEN_ALL evaluate_add_clock_io_events_mono) \\
+    simp[Abbr`ss`]) >>
+  simp[equiv_lprefix_chain_thm] >>
+  unabbrev_all_tac >> simp[PULL_EXISTS] >>
+  ntac 2 (pop_assum kall_tac) >>
+  simp[LNTH_fromList,PULL_EXISTS] >>
+  simp[GSYM FORALL_AND_THM] >>
+  rpt gen_tac >>
+  (fn g => subterm (fn tm => Cases_on`^(assert has_pair_type tm)`) (#2 g) g) >> full_simp_tac(srw_ss())[] >>
+  (fn g => subterm (fn tm => Cases_on`^(assert (fn tm => has_pair_type tm andalso free_in tm (#2 g)) tm)`) (#2 g) g) >> full_simp_tac(srw_ss())[] >>
+  drule comp_correct_thm >>
+  simp[comp_def,RIGHT_FORALL_IMP_THM] >>
+  impl_tac >- (
+    simp[alloc_arg_def] >>
+    reverse conj_tac >- metis_tac[] >>
+    rpt(first_x_assum(qspec_then`k`mp_tac))>>srw_tac[][] ) >>
+  strip_tac >>
+  reverse conj_tac >- (
+    srw_tac[][] >>
+    qexists_tac`ck+k`>>simp[] ) >>
+  srw_tac[][] >>
+  qexists_tac`k`>>simp[] >>
+  ntac 2 (qhdtm_x_assum`evaluate`mp_tac) >>
+  qmatch_assum_abbrev_tac`evaluate (e,ss) = _` >>
+  Q.ISPECL_THEN[`ck`,`e`,`ss`]mp_tac(GEN_ALL evaluate_add_clock_io_events_mono)>>
+  simp[Abbr`ss`] >>
+  ntac 3 strip_tac >> full_simp_tac(srw_ss())[] >>
+  full_simp_tac(srw_ss())[IS_PREFIX_APPEND] >>
+  simp[EL_APPEND1]
+QED
+
+(* TODO: does this have to initialize the data_buffer to empty? *)
+val make_init_def = Define `
+  make_init c code oracle s =
+    s with <| code := code; use_alloc := T; use_stack := T; gc_fun := word_gc_fun c
+            ; compile := λc. s.compile c o (MAP prog_comp)
+            ; compile_oracle := oracle |>`;
+
+Theorem prog_comp_lambda:
+   prog_comp = λ(n,p). ^(rhs (concl (SPEC_ALL prog_comp_def)))
+Proof
+  srw_tac[][FUN_EQ_THM,prog_comp_def,LAMBDA_PROD,FORALL_PROD]
+QED
+
+Theorem make_init_semantics:
+   (!k prog. ALOOKUP code k = SOME prog ==> k <> gc_stub_location /\ alloc_arg prog) /\
+   (∀n k p.  MEM (k,p) (FST (SND (oracle n))) ⇒ k ≠ gc_stub_location ∧ alloc_arg p) /\
+   s.use_stack ∧ s.use_store ∧ ~s.use_alloc /\ s.code = fromAList (compile c code) /\
+   s.compile_oracle = (I ## MAP prog_comp ## I) o oracle /\
+   LENGTH s.bitmaps + LENGTH s.data_buffer.buffer + s.data_buffer.space_left < dimword (:α) − 1 ∧
+   LENGTH s.stack * (dimindex (:α) DIV 8) < dimword (:α) ∧
+   ALL_DISTINCT (MAP FST code) /\
+   semantics start (make_init c (fromAList code) oracle s) <> Fail ==>
+   semantics start (s:('a,'c,'ffi) stackSem$state) =
+   semantics start (make_init c (fromAList code) oracle s)
+Proof
+  srw_tac[][]
+  \\ drule (CONV_RULE(LAND_CONV(move_conj_left(can dest_neg)))compile_semantics
+            |> GEN_ALL)
+  \\ disch_then (qspecl_then [`s.compile`,`c`,`s.gc_fun`] mp_tac)
+  \\ full_simp_tac(srw_ss())[make_init_def,lookup_fromAList]
+  \\ impl_tac THEN1 (srw_tac[][] \\ res_tac \\ full_simp_tac(srw_ss())[])
+  \\ disch_then (assume_tac o GSYM)
+  \\ full_simp_tac(srw_ss())[] \\ AP_TERM_TAC
+  \\ full_simp_tac(srw_ss())[state_component_equality]
+  \\ full_simp_tac(srw_ss())[spt_eq_thm,wf_fromAList,lookup_fromAList,compile_def]
+  \\ srw_tac[][]
+  \\ srw_tac[][ALOOKUP_APPEND] \\ BasicProvers.CASE_TAC
+  \\ simp[prog_comp_lambda,ALOOKUP_MAP_2]
+  \\ simp[ALOOKUP_toAList,lookup_fromAList]
+QED
+
+Theorem next_lab_EQ_MAX = Q.prove(`
+  !q (n:num) aux. next_lab q aux = MAX aux (next_lab q 0)`,
+  ho_match_mp_tac next_lab_ind>>Cases_on`q`>>rw[]>>
+  once_rewrite_tac [next_lab_def]>>
+  simp_tac (srw_ss()) [] >>
+  every_case_tac >>
+  simp_tac (srw_ss()) [] >>
+  rpt (qpat_x_assum `!x. _` (mp_tac o SIMP_RULE std_ss [])) >>
+  rpt strip_tac >>
+  rpt (pop_assum (fn th => once_rewrite_tac [th])) >>
+  fs [AC MAX_ASSOC MAX_COMM]) |> SIMP_RULE std_ss [];
+
+val MAX_SIMP = prove(
+  ``MAX n (MAX n m) = MAX n m``,
+  fs [MAX_DEF]);
+
+Theorem next_lab_thm:
+   !p.
+      next_lab (p:'a stackLang$prog) 2 =
+      case p of
+      | Seq p1 p2 => MAX (next_lab p1 2) (next_lab p2 2)
+      | If _ _ _ p1 p2 => MAX (next_lab p1 2) (next_lab p2 2)
+      | While _ _ _ p => next_lab p 2
+      | Call NONE _ NONE => 2
+      | Call NONE _ (SOME (_,_,l2)) => MAX (l2 + 2) 2
+      | Call (SOME (p,_,_,l2)) _ NONE => MAX (next_lab p 2) (l2 + 2)
+      | Call (SOME (p,_,_,l2)) _ (SOME (p',_,l3)) =>
+           MAX (MAX (next_lab p 2) (next_lab p' 2)) (MAX l2 l3 + 2)
+      | _ => 2
+Proof
+  Induct \\ simp [Once next_lab_def] \\ fs []
+  \\ once_rewrite_tac [next_lab_EQ_MAX]
+  \\ once_rewrite_tac [next_lab_EQ_MAX]
+  \\ once_rewrite_tac [next_lab_EQ_MAX]
+  \\ fs [AC MAX_ASSOC MAX_COMM,MAX_SIMP]
+  \\ every_case_tac \\ fs []
+  \\ once_rewrite_tac [next_lab_EQ_MAX]
+  \\ once_rewrite_tac [next_lab_EQ_MAX]
+  \\ once_rewrite_tac [next_lab_EQ_MAX]
+  \\ fs [AC MAX_ASSOC MAX_COMM,MAX_SIMP]
+  \\ fs [MAX_DEF]
+QED
+
+Theorem extract_labels_next_lab:
+    ∀p (aux:num) e.
+    MEM e (extract_labels p) ⇒
+    SND e < next_lab p 2
+Proof
+  ho_match_mp_tac next_lab_ind>>Cases_on`p`>>rw[]>>
+  once_rewrite_tac [next_lab_thm]>>fs[extract_labels_def]>>
+  fs[extract_labels_def]>>
+  BasicProvers.EVERY_CASE_TAC>>fs []>>fs[MAX_DEF]
+QED
+
+Theorem stack_alloc_lab_pres:
+    ∀n nl p aux.
+  EVERY (λ(l1,l2). l1 = n ∧ l2 ≠ 0 ∧ l2 ≠ 1) (extract_labels p) ∧
+  ALL_DISTINCT (extract_labels p) ∧
+  next_lab p 2 ≤ nl ⇒
+  let (cp,nl') = comp n nl p in
+  EVERY (λ(l1,l2). l1 = n ∧ l2 ≠ 0 ∧ l2 ≠ 1) (extract_labels cp) ∧
+  ALL_DISTINCT (extract_labels cp) ∧
+  (∀lab. MEM lab (extract_labels cp) ⇒ MEM lab (extract_labels p) ∨ (nl ≤ SND lab ∧ SND lab < nl')) ∧
+  nl ≤ nl'
+Proof
+  HO_MATCH_MP_TAC comp_ind>>Cases_on`p`>>rw[]>>
+  once_rewrite_tac [comp_def]>>fs[extract_labels_def]
+  >-
+    (BasicProvers.EVERY_CASE_TAC>>fs[]>>rveq>>fs[extract_labels_def]>>
+    rpt(pairarg_tac>>fs[])>>rveq>>fs[extract_labels_def]>>
+    qpat_x_assum`A<=nl` mp_tac>>
+    simp[Once next_lab_thm]>>
+    strip_tac>>
+    fs[ALL_DISTINCT_APPEND]
+    >-
+      (CCONTR_TAC>>fs[]>>
+      res_tac>>fs[])
+    >>
+      `next_lab q 2 ≤ m'` by fs[]>>
+      fs[]>>rfs[]>>
+      `r < nl ∧ r' < nl` by
+        fs[MAX_DEF]>>
+      rw[]>>
+      TRY(CCONTR_TAC>>fs[]>>
+      res_tac>>fs[])
+      >- metis_tac[]
+      >>
+        imp_res_tac extract_labels_next_lab>>fs[])
+  >>
+  TRY
+  (rpt(pairarg_tac>>fs[])>>rveq>>fs[extract_labels_def]>>
+  qpat_x_assum`A<=nl` mp_tac>>
+  simp[Once next_lab_thm])>>
+  (strip_tac>>
+  fs[ALL_DISTINCT_APPEND]>>rw[]
+  >-
+    (CCONTR_TAC>>fs[]>>
+    res_tac>>fs[]>- metis_tac[]>>
+    imp_res_tac extract_labels_next_lab>>
+    fs[])
+  >>
+    res_tac>>fs[])
+QED
+
+Theorem stack_alloc_comp_stack_asm_name:
+    ∀n m p.
+  stack_asm_name c p ∧ stack_asm_remove (c:'a asm_config) p ⇒
+  let (p',m') = comp n m p in
+  stack_asm_name c p' ∧ stack_asm_remove (c:'a asm_config) p'
+Proof
+  ho_match_mp_tac comp_ind>>Cases_on`p`>>rw[]>>
+  simp[Once comp_def]
+  >-
+    (Cases_on`o'`>-
+      fs[Once comp_def,stack_asm_name_def,stack_asm_remove_def]
+    >>
+    PairCases_on`x`>>SIMP_TAC std_ss [Once comp_def]>>fs[]>>
+    FULL_CASE_TAC>>fs[]>>
+    TRY(PairCases_on`x`)>>
+    rpt(pairarg_tac>>fs[])>>rw[]>>
+    fs[stack_asm_name_def,stack_asm_remove_def])
+  >>
+    rpt(pairarg_tac>>fs[])>>rw[]>>
+    fs[stack_asm_name_def,stack_asm_remove_def]
+QED
+
+Theorem stack_alloc_stack_asm_convs:
+    EVERY (λ(n,p). stack_asm_name c p) prog ∧
+  EVERY (λ(n,p). (stack_asm_remove (c:'a asm_config) p)) prog ∧
+  (* conf_ok is too strong, but we already have it anyway *)
+  conf_ok (:'a) conf ∧
+  addr_offset_ok c 0w ∧
+  reg_name 10 c ∧ good_dimindex(:'a) ∧
+  c.valid_imm (INL Add) 8w ∧
+  c.valid_imm (INL Add) 4w ∧
+  c.valid_imm (INL Add) 1w ∧
+  c.valid_imm (INL Sub) 1w
+  ⇒
+  EVERY (λ(n,p). stack_asm_name c p) (compile conf prog) ∧
+  EVERY (λ(n,p). stack_asm_remove c p) (compile conf prog)
+Proof
+  fs[compile_def]>>rw[]>>
+    TRY (EVAL_TAC>>every_case_tac >>
+         EVAL_TAC>>every_case_tac >>
+         fs [] >> EVAL_TAC >>
+     fs[reg_name_def, labPropsTheory.good_dimindex_def,
+        asmTheory.offset_ok_def, data_to_wordTheory.conf_ok_def,
+        data_to_wordTheory.shift_length_def]>>
+     pairarg_tac>>fs[]>>NO_TAC)
+  >>
+  fs[EVERY_MAP,EVERY_MEM,FORALL_PROD,prog_comp_def]>>
+  rw[]>>res_tac>>
+  drule stack_alloc_comp_stack_asm_name>>fs[]>>
+  disch_then(qspecl_then[`p_1`,`next_lab p_2 2`] assume_tac)>>
+  pairarg_tac>>fs[]
+QED
+
+Theorem stack_alloc_reg_bound:
+   10 ≤ sp ∧
+    EVERY (\p. reg_bound p sp)
+       (MAP SND prog1) ==>
+    EVERY (\p. reg_bound p sp)
+       (MAP SND (compile dc prog1))
+Proof
+  fs[stack_allocTheory.compile_def]>>
+  strip_tac>>CONJ_TAC
+  >-
+    (EVAL_TAC>>TOP_CASE_TAC>>EVAL_TAC>>fs[]>>
+    IF_CASES_TAC>>EVAL_TAC>>fs[])
+  >>
+  pop_assum mp_tac>>
+  qid_spec_tac`prog1`>>Induct>>
+  fs[stack_allocTheory.prog_comp_def,FORALL_PROD]>>
+  ntac 3 strip_tac>>fs[]>>
+  qpat_x_assum`reg_bound p_2 sp` mp_tac>>
+  qpat_x_assum`10 ≤ sp` mp_tac>>
+  rpt (pop_assum kall_tac)>>
+  (qpat_abbrev_tac`l = next_lab _ _`) >> pop_assum kall_tac>>
+  qid_spec_tac `p_2` >>
+  qid_spec_tac `l` >>
+  qid_spec_tac `p_1` >>
+  ho_match_mp_tac stack_allocTheory.comp_ind>>
+  Cases_on`p_2`>>rw[]>>
+  simp[Once stack_allocTheory.comp_def]>>
+  fs[reg_bound_def]>>
+  TRY(ONCE_REWRITE_TAC [stack_allocTheory.comp_def]>>
+    Cases_on`o'`>>TRY(PairCases_on`x`)>>fs[reg_bound_def]>>
+    BasicProvers.EVERY_CASE_TAC)>>
+  rpt(pairarg_tac>>fs[reg_bound_def])
+QED
+
+Theorem stack_alloc_call_args:
+   EVERY (λp. call_args p 1 2 3 4 0) (MAP SND prog1) ==>
+   EVERY (λp. call_args p 1 2 3 4 0) (MAP SND (compile dc prog1))
+Proof
+  fs[stack_allocTheory.compile_def]>>
+  strip_tac>>CONJ_TAC
+  >-
+    (EVAL_TAC>>TOP_CASE_TAC>>EVAL_TAC>>fs[]>>
+    IF_CASES_TAC>>EVAL_TAC>>fs[])
+  >>
+  pop_assum mp_tac>>
+  qid_spec_tac`prog1`>>Induct>>
+  fs[stack_allocTheory.prog_comp_def,FORALL_PROD]>>
+  ntac 3 strip_tac>>fs[]>>
+  (qpat_abbrev_tac`l = next_lab _ _`) >> pop_assum kall_tac>>
+  qpat_x_assum`call_args p_2 1 2 3 4 0` mp_tac>>
+  rpt (pop_assum kall_tac)>>
+  qid_spec_tac `p_2` >>
+  qid_spec_tac `l` >>
+  qid_spec_tac `p_1` >>
+  ho_match_mp_tac stack_allocTheory.comp_ind>>
+  Cases_on`p_2`>>rw[]>>
+  simp[Once stack_allocTheory.comp_def]>>fs[call_args_def]>>
+  TRY(ONCE_REWRITE_TAC [stack_allocTheory.comp_def]>>
+    Cases_on`o'`>>TRY(PairCases_on`x`)>>fs[call_args_def]>>
+    BasicProvers.EVERY_CASE_TAC)>>
+  rpt(pairarg_tac>>fs[call_args_def])
+QED
+
+Theorem compile_has_fp_ops[simp]:
+  compile (dconf with <| has_fp_ops := b1; has_fp_tern := b2 |>) code = compile dconf code
+Proof
+  fs [compile_def,stubs_def,word_gc_code_def]
+  \\ every_case_tac \\ fs []
+  \\ fs [data_to_wordTheory.small_shift_length_def,
+         word_gc_move_code_def,
+         word_gc_move_list_code_def,
+         word_gc_move_loop_code_def,
+         word_gc_move_roots_bitmaps_code_def,
+         word_gc_move_bitmaps_code_def,
+         word_gc_move_bitmap_code_def,
+         word_gen_gc_move_code_def,
+         word_gen_gc_move_list_code_def,
+         word_gen_gc_move_roots_bitmaps_code_def,
+         word_gen_gc_move_bitmaps_code_def,
+         word_gen_gc_move_bitmap_code_def,
+         word_gen_gc_move_data_code_def,
+         word_gen_gc_move_refs_code_def,
+         word_gen_gc_move_loop_code_def,
+         word_gen_gc_partial_move_code_def,
+         word_gen_gc_partial_move_list_code_def,
+         word_gen_gc_partial_move_roots_bitmaps_code_def,
+         word_gen_gc_partial_move_bitmaps_code_def,
+         word_gen_gc_partial_move_bitmap_code_def,
+         word_gen_gc_partial_move_data_code_def,
+         word_gen_gc_partial_move_ref_list_code_def]
+QED
+
+*)
+
+val _ = export_theory();
