compiler/backend/stack_rawcallScript.sml
@@ -1,0 +1,108 @@
+(*
+  This compiler phase introduces calls past the stack allocation code
+  that is present at almost every start of function. A call past stack
+  allocation is called a RawCall. RawCalls are introduced to shortcut
+  some bookkeeping during tail-calls to known locations, i.e
+  `Call NONE (INL dest) ..`.
+*)
+open preamble stackLangTheory data_to_wordTheory;
+
+val _ = new_theory "stack_rawcall";
+
+val _ = patternMatchesLib.ENABLE_PMATCH_CASES();
+
+(* collect stack allocation information *)
+
+Definition seq_stack_alloc_def:
+  seq_stack_alloc (p: 'a stackLang$prog) =
+    dtcase p of Seq (StackAlloc k) _ => SOME k | _ => NONE
+End
+
+Theorem seq_stack_alloc_pmatch:
+  seq_stack_alloc (p: 'a stackLang$prog) =
+    case p of Seq (StackAlloc k) _ => SOME k | _ => NONE
+Proof
+  CONV_TAC(patternMatchesLib.PMATCH_LIFT_BOOL_CONV true) \\ rw []
+  \\ rw[Once seq_stack_alloc_def,pairTheory.ELIM_UNCURRY] \\ every_case_tac \\ fs[]
+QED
+
+Definition collect_info_def:
+  (collect_info [] f = f) /\
+  (collect_info ((n,b:'a stackLang$prog)::xs) f =
+     collect_info xs (dtcase seq_stack_alloc b of
+                      | NONE => f
+                      | SOME k => insert n k f))
+End
+
+(* optimise based on stack allocation information *)
+
+Definition dest_case_def:
+  dest_case (p: 'a stackLang$prog # 'a stackLang$prog) =
+    dtcase p of (StackFree k, Call NONE (INL d) _) => SOME (k,d) | _ => NONE
+End
+
+Theorem dest_case_pmatch:
+  dest_case (p: 'a stackLang$prog # 'a stackLang$prog) =
+    case p of (StackFree k, Call NONE (INL d) _) => SOME (k,d) | _ => NONE
+Proof
+  CONV_TAC(patternMatchesLib.PMATCH_LIFT_BOOL_CONV true) \\ rw []
+  \\ rw[Once dest_case_def,pairTheory.ELIM_UNCURRY] \\ every_case_tac \\ fs[]
+QED
+
+Definition comp_seq_def:
+  comp_seq (p1:'a stackLang$prog) (p2:'a stackLang$prog) i (default:'a stackLang$prog) =
+  dtcase dest_case (p1,p2) of
+  | SOME (k,dest) =>
+      (dtcase lookup dest i of
+       | NONE => default
+       | SOME l =>
+           if l = k then RawCall dest else
+           if l < k then Seq (StackFree (k - l)) (RawCall dest) else
+               Seq Tick (Seq (StackAlloc (l - k)) (RawCall dest)))
+  | _ => default
+End
+
+local
+val q = `
+  comp i (p:'a stackLang$prog) =
+    dtcase p of
+    | Seq p1 p2 => comp_seq p1 p2 i (Seq (comp i p1) (comp i p2))
+    | If c r ri p1 p2 => If c r ri (comp i p1) (comp i p2)
+    | While c r ri p1 => While c r ri (comp i p1)
+    | Call (SOME (p1,lr,l1,l2)) dest NONE =>
+        Call (SOME (comp i p1,lr,l1,l2)) dest NONE
+    | Call (SOME (p1,lr,l1,l2)) dest (SOME (p2,k1,k2)) =>
+        Call (SOME (comp i p1,lr,l1,l2)) dest NONE
+    | _ => p`
+in
+val comp_def = Define q;
+Theorem comp_pmatch = Q.prove(
+  `∀i p.` @
+    (map (fn QUOTE s => Portable.replace_string {from="dtcase",to="case"} s |> QUOTE
+         | aq => aq) q),
+  rpt strip_tac
+  \\ CONV_TAC(patternMatchesLib.PMATCH_LIFT_BOOL_CONV true) \\ rw []
+  \\ rw[Once comp_def,pairTheory.ELIM_UNCURRY] \\ every_case_tac \\ fs[]
+  \\ rename [`NONE = opt`] \\ Cases_on `opt` \\ fs [] \\ metis_tac [PAIR]);
+end
+
+Definition comp_top_def:
+  comp_top i (p: 'a stackLang$prog) =
+    dtcase p of Seq p1 p2 => Seq (comp i p1) (comp i p2) | _ => comp i p
+End
+
+Theorem comp_top_pmatch:
+  comp_top i (p: 'a stackLang$prog) =
+    case p of Seq p1 p2 => Seq (comp i p1) (comp i p2) | _ => comp i p
+Proof
+  CONV_TAC(patternMatchesLib.PMATCH_LIFT_BOOL_CONV true) \\ rw []
+  \\ rw[Once comp_top_def,pairTheory.ELIM_UNCURRY] \\ every_case_tac \\ fs[]
+QED
+
+Definition compile_def:
+  compile prog =
+    let i = collect_info prog LN in
+      MAP (\(n,b:'a stackLang$prog). (n,comp_top i b)) prog
+End
+
+val _ = export_theory();
